Update Tangles_update.thy

Tangles_update.thy
@@ -1604,7 +1604,7 @@ done
 
 lemma makestrand_fstsndequality:"(fst (count (makestrand n))) = (snd (count (makestrand n)))" 
 apply (induct_tac n)
-apply(auto)
+apply(auto simp add:e1_def)
 done
 
 lemma nat_int:" ((int n)≥ 0)" by auto
@@ -1615,21 +1615,8 @@ by auto
 lemma strands_even: "((a = Abs_diagram (x ∘(basic y)∘ z)) ∧ (strands y)) ⟹ (length y) > 1"
 proof-
 oops
-(*
-definition P_compress_rightcenter::"walls=>block=>block=>block=>block=>walls=>bool"
-where
-"P_compress_rightcenter y1 w1 w2 A B y2 ≡ ((a = Abs_diagram
- ((y1)∘(basic (A⊗w1))∘(basic (B⊗w2))∘(y2)))∧ (b = Abs_diagram ((y1)∘
-(basic (w1))∘(basic (A⊗w2))∘(y2)))
-∧((snd (count w1)) = (fst (count w2)))
-∧((fst (count A)) = 0))
-∧(strands B)" 
 
-lemma P_tanglerel: 
-" tanglerel_compbelow_centerright x y 
-≡ ∃y1.∃w1.∃w2.∃A.∃B.∃y2.(P_compress_rightcenter y1 w1 w2 A B y2)" 
-using  tanglerel_compbelow_centerright_def P_compress_rightcenter_def 
-*)
+
 theorem metaequivalence_left: 
 "((strands z2) ∧ (strands z3))∧((snd (count y1))>1)∧(tanglerel_equiv (Abs_diagram (x1∘(basic y1)∘z1))  
 (Abs_diagram ((x1)∘(basic (e2⊗y1))∘
@@ -1674,74 +1661,66 @@ have subresult7: "snd (count y1) = int(k)+2"
 have subresult8: "fst (count (z4)) = (snd (count y1))" 
            using subresult5 subresult7 
            by auto
-(*
-have subresult_main1: 
+have subresult_compress1: 
 "(tanglerel_compress_null ((Abs_diagram (x2∘(basic z4)∘z1))) (Abs_diagram (x2∘z1)))" 
-           using tanglerel_compress_null_def preliminary_result3 subresult0 subresult2
-           by metis
-
-have subresult_main2: 
-"tanglerel_equiv (Abs_diagram (x2∘z1)) ((Abs_diagram (x2∘basic z4∘z1))) "
-          using tanglerel_equiv_def tanglerel_def tanglerel_compress_def subresult_main1 
-r_into_rtranclp
-          by (metis (full_types)
-)
-assume F: "x3 = x2 ∘ basic z4" 
-
-have subresult_main3: "tanglerel_equiv (Abs_diagram (x2∘z1)) ((Abs_diagram (x3∘z1))) "
-          using subresult_main2  compose_leftassociativity F 
-          by auto
-*)
-(*
-have subresult_tanglerel1_mod:  
-
-
-have subresult3: "(snd (wall_count x3)) = (snd (wall_count (basic z4)))" 
-           using wall_count_compose F
-                  by auto
-have subresult4: "(snd (wall_count (basic z4))) = (snd (count z4))" using wall_count_def by auto
-have subresult5: "(snd (count z4)) = (fst (count z4))" 
-               using C makestrand_fstsndequality by auto
-have subresult6: "(snd (wall_count x3))>0" 
-               using C subresult3 subresult4 subresult5 
-               makestrands_positivelength by metis
-
-have subresult_main2:"(tanglerel_compress_null ((Abs_diagram (x3∘(basic z4)∘z1))) 
-(Abs_diagram (x3∘z1)))" 
-   using  subresult subresult2 F tanglerel_compress_null_def subresult0 subresult6 
-           by auto
-
-have subresult_tanglerel2:"(tanglerel_equiv (Abs_diagram (x3∘z1))
- (Abs_diagram (x3∘(basic z4)∘z1))) " using tanglerel_def tanglerel_compress_def subresult_main2 tanglerel_equiv_def
-by (metis (full_types) r_into_rtranclp)
-
-have subresult_main3:
-"tanglerel_equiv (Abs_diagram (x2∘z1)) (Abs_diagram (x3∘(basic z4)∘z1)) "
-using subresult_tanglerel1_mod subresult_tanglerel2 rtranclp_trans E by (metis Tangle.abs_eq_iff)
-*)
+           using tanglerel_compress_null_def
+           preliminary_result3 subresult0 subresult2
+             by metis
+have subresult_equiv1: 
+"(tanglerel_equiv ((Abs_diagram (x2∘(basic z4)∘z1))) (Abs_diagram (x2∘z1)))" 
+           using r_into_rtranclp subresult_compress1 tanglerel_equiv_def tanglerel_def  
+           tanglerel_compress_def
+                     by (metis)
+have subresult_compress2: 
+"(tanglerel_compress_null ((Abs_diagram ((x2 ∘ basic z4)∘(basic z4)∘z1))) 
+                            (Abs_diagram ((x2 ∘ basic z4)∘z1)))" 
+               using tanglerel_compress_null_def preliminary_result3 subresult0 subresult2   
+               compose_leftassociativity
+                    by (fastforce)
+have subresult_equiv2: 
+"(tanglerel_equiv ((Abs_diagram ((x2 ∘ basic z4)∘(basic z4)∘z1))) 
+                            (Abs_diagram ((x2 ∘ basic z4)∘z1)))" 
+               using tanglerel_compress_def tanglerel_def tanglerel_equiv_def
+               r_into_rtranclp subresult_compress2   
+                    by (metis)
+have subresult_equiv3: 
+"tanglerel_equiv ((Abs_diagram ((x2 ∘ basic z4)∘(basic z4)∘z1))) 
+                            (Abs_diagram ((x2 ∘z1)))" 
+               using tanglerel_equiv_def rtranclp_trans subresult_equiv1 subresult_equiv2 
+               compose_leftassociativity
+                            by (metis) 
+have step1: 
+"tanglerel_equiv (Abs_diagram (x1 ∘ basic y1 ∘ basic z4∘basic z4∘z1)) 
+                            (Abs_diagram (x1 ∘ basic y1 ∘z1))" 
+               using compose_leftassociativity subresult_equiv3 E
+               by auto
 (*step 2 - inducing cusp*)
+
+assume w_subst: "w4 = (makestrand k)"
 
 have step2_subresult0: "(makestrand (k+1)) = (e1⊗(makestrand k))" 
  apply(simp add: e1_def)
  done
 
-have step2_subresult1:"z4 = e1⊗(makestrand k)" using O A step2_subresult0 by metis
+have step2_subresult1:"z4 = e1⊗(makestrand k)" using A C step2_subresult0 by auto
 
-assume w_subst: "w4 = (makestrand k)"
 have step2_subresult2: "(Abs_diagram (x2 ∘ (basic z4) ∘(basic z4)∘z1)) =
-(Abs_diagram (x2  ∘ (basic (e1⊗w4))∘
-(basic (e1 ⊗w4))∘z1))" using w_subst step2_subresult1 by auto
+(Abs_diagram (x2  ∘ (basic (e1⊗w4))∘ (basic (e1 ⊗w4))∘z1))" 
+                        using w_subst step2_subresult1 by auto
+
 have step2_subresult3: "(snd (count w4)) = (fst (count w4))" using makestrand_fstsndequality w_subst
 by auto
+
 assume temp_a: "x = (Abs_diagram (x2 ∘(basic (e2⊗e1⊗w4))∘(basic (e1⊗e3⊗w4))∘z1))"
 assume temp_b: "y = (Abs_diagram (x2 ∘(basic (e1⊗w4))∘(basic (e1⊗w4))∘z1))"
 
 have step2_subresult4:
 "∃y1.∃y2.∃w1.∃w2.(x = Abs_diagram (y1 ∘ (basic (e2 ⊗ e1 ⊗ w1)) ∘ (basic (e1 ⊗ e3 ⊗ w2)) ∘ y2))"
- using temp_a by auto
+  using temp_a exI by auto
+ 
 have step2_subresult5:
 "∃y1.∃y2.∃w1.∃w2.(y = Abs_diagram (y1 ∘ (basic (e1 ⊗ w1)) ∘ (basic (e1 ⊗ w2)) ∘ y2))"
- using temp_b by auto
+ using temp_b exI by auto
 
 have step2_subresult6: 
 " (∃y1.∃w1.∃w2.∃y2.((x = Abs_diagram ((y1)
@@ -1749,116 +1728,115 @@ have step2_subresult6:
  ((y1)
 ∘(basic (e1⊗w1))∘(basic (e1⊗w2))∘(y2))))
  ∧ ((snd (count w1)) = (fst (count w2))))"
-using temp_a temp_b step2_subresult3 sorry
+using temp_a temp_b step2_subresult3 exI by auto
 
-have step2_subresult:
+have step2_subresult7:
 " tanglerel_straighten_rightdowntop x y"
 using tanglerel_straighten_rightdowntop_def step2_subresult6 by auto
 
-have step2_subresult7:"tanglerel y x" 
-using tanglerel_def tanglerel_straighten_def step2_subresult by auto
+have step2_subresult8:"tanglerel x y" 
+using tanglerel_def tanglerel_straighten_def step2_subresult7 by auto
 
+have step2_subresult9: "tanglerel (Abs_diagram (x2 ∘(basic (e2⊗e1⊗w4))∘(basic (e1⊗e3⊗w4))∘z1)) 
+              (Abs_diagram (x2 ∘(basic (e1⊗w4))∘(basic (e1⊗w4))∘z1))"
+               using temp_a temp_b step2_subresult8 by auto
+
+have step2_equiv1: "tanglerel_equiv (Abs_diagram (x1∘basic y1∘(basic (e2⊗e1⊗w4))∘(basic (e1⊗e3⊗w4))∘z1)) 
+              (Abs_diagram (x1∘basic y1 ∘(basic (e1⊗w4))∘(basic (e1⊗w4))∘z1))"
+               using temp_a temp_b E step2_subresult9 compose_leftassociativity r_into_rtranclp 
+               tanglerel_equiv_def
+                     by metis
+
+have step2: "tanglerel_equiv (Abs_diagram (x1∘basic y1∘(basic (e2⊗z4))∘(basic (e1⊗e3⊗w4))∘z1)) 
+              (Abs_diagram (x1∘basic y1 ∘(basic z4)∘(basic (z4))∘z1))"
+               using temp_a temp_b E step2_subresult9 compose_leftassociativity r_into_rtranclp 
+               tanglerel_equiv_def step2_subresult1 w_subst
+                     by (metis)
 (*step 3*)
-have step3_subresult1 :"fst (wall_count (basic (e1⊗w4))) = fst (wall_count (basic (e2⊗e1⊗w4)))" by auto
+
+have step3_preliminary1: "fst (count (v⊗w)) = fst (count (a2#(v⊗w)))" using count_def brickcount_def
+by auto
+have step3_subresult0 : "fst (count (a2#(e2⊗w4))) = (fst (brickcount (a2))) +(fst (count (e1⊗w4)))"
+using count_def append_def sorry
+
+have step3_subresult1 :"fst (wall_count (basic (e1⊗w4))) = fst (wall_count (basic (e2⊗e1⊗w4)))" 
+using wall_count_def sorry
 have step3_subresult2: "fst (wall_count (basic (e1⊗w4))) = snd (count y1)" 
                using w_subst step2_subresult1 subresult8 by auto
 have step3_subresult3: "fst (wall_count (basic (e2⊗e1⊗w4))) = snd (count y1)" 
                using step3_subresult1 step3_subresult2 by auto 
 have step3_subresult4: "fst (wall_count (basic (e1⊗w4))) = snd (wall_count x2)" 
-               using step3_subresult3 subresult1 by auto 
+               using step3_subresult3 subresult0 wall_count_def step3_subresult2 subresult1 by auto 
 have step3_subresult5: "fst (wall_count (basic (e1⊗w4))) = snd (wall_count (x1∘(basic y1)))" 
-               using step3_subresult4 D wall_count_def by auto
+               using step3_subresult4 E  wall_count_def by auto
+have step3_subresult6: "fst (brickcount a2) =  0" using brickcount_def by auto
+have step3_subresult7: "fst (count e2) =  0" using e2_def count_def step3_subresult6 
+by (metis count.simps(1))
+have step3_subresult8: "strands (a1#e1)" using e1_def append_def strands_def  brickstrand.simps(1) 
+                        strands.simps(1) strands.simps(2) 
+                       by metis
+have step3_subresult9: "(a1#e1) = (e1⊗e1)" using append_Nil e1_def
+                        by metis
+have step3_subresult10: "strands (e1⊗e1)" using step3_subresult8 step3_subresult9
+                        by auto
+assume temp: " a0 = (basic (e1⊗e3⊗w4))∘z1"
+assume temp_w: "b0 = e1⊗e1"
+assume temp_x:  "a =  Abs_diagram ((x1)∘(basic (e2⊗y1))∘(basic (b0⊗(e1⊗w4)))∘a0)"
+assume temp_y: "b = Abs_diagram (((x1)∘(basic y1))∘(basic (e2 ⊗ (e1 ⊗ w4)))∘ a0)"
 
-have step3_subresult6: "fst (count e2) = 0" by auto
-have step3_subresult7: "strands (e1 ⊗ e1)" by auto
-assume temp: " p = (basic (e1⊗e3⊗w5))∘z1"
+have step3_subresult11: "  ∃y1.∃w1.∃w2.∃A.∃B.∃y2.(a = Abs_diagram
+ ((y1)∘(basic (A⊗w1))∘(basic (B⊗w2))∘(y2)))"
+using temp_x exI by metis
 
-assume temp_w: "a0 = e1⊗e1"
-assume temp_x:  "a =  Abs_diagram ((x1)∘(basic (e2⊗y1))∘(basic (a0⊗e1⊗w4))∘p)"
-assume temp_y: "b = Abs_diagram ((x1)∘(basic y1)∘(basic (e2 ⊗ e1 ⊗ w1))∘ p)"
+have step3_subresult12: " ∃y1.∃w1.∃w2.∃A.∃B.∃y2.(b = Abs_diagram
+ ((y1)∘(basic (w1))∘(basic (A⊗w2))∘(y2)))"
+using temp_y temp exI 
+by metis
 
-have step3_subresult8: "  ∃y1.∃w1.∃w2.∃A.∃B.∃y2.((a = Abs_diagram
- ((y1)∘(basic (A⊗w1))∘(basic (B⊗w2))∘(y2)))∧ (b = Abs_diagram ((y1)∘
-(basic (w1))∘(basic (A⊗w2))∘(y2)))
+have step3_subresult13: "  ∃y1.∃w1.∃w2.∃A.∃B.∃y2.(a = Abs_diagram
+ ((y1)∘(basic (A⊗w1))∘(basic (B⊗w2))∘(y2)) ∧
+ (b = Abs_diagram
+ ((y1)∘(basic (w1))∘(basic (A⊗w2))∘(y2)))
 ∧((snd (count w1)) = (fst (count w2)))
 ∧((fst (count A)) = 0)
-∧(strands B))" using temp_w temp_x temp_y step3_subresult5 step3_subresult6  step3_subresult7 
-sorry
-
-have step3_subresult9: "tanglerel_compbelow_centerright a b" using step3_subresult8 
+∧(strands B))" 
+using temp_w temp_x temp_y 
+step3_subresult11 step3_subresult12
+compose_leftassociativity step2_subresult1 subresult8 w_subst
+step3_subresult5 step3_subresult7 step3_subresult10 exI
+by (metis)
+have step3_subresult14: "tanglerel_compbelow_centerright a b" using step3_subresult13 
 tanglerel_compbelow_centerright_def by auto
-
-have step3_subresult10: "tanglerel_compress a b" using step3_subresult9 tanglerel_compress_def 
+have step3_subresult15: "tanglerel_compress a b" using step3_subresult14 tanglerel_compress_def 
 tanglerel_compbelow_def by auto
-
-
-have step3_subresult11: "tanglerel a b" using step3_subresult10 tanglerel_def by auto
-
-
-have step3_subresult11: "tanglerel_equiv a b"
-    using step3_subresult11 tanglerel_equiv_def r_into_rtranclp
+have step3_subresult16: "tanglerel a b" using step3_subresult15 tanglerel_def by auto
+have step3_subresult17: "tanglerel_equiv a b"
+    using step3_subresult16 tanglerel_equiv_def r_into_rtranclp
        by (metis (full_types) r_into_rtranclp)
 
-have step3_subresult12: "tanglerel_equiv (Abs_diagram ((x1)∘(basic (e2⊗y1))∘(basic (a0⊗e1⊗w4))∘p)) 
- (Abs_diagram ((x1)∘(basic y1)∘(basic (e2 ⊗ e1 ⊗ w1))∘ p))" using step3_subresult11 temp_x temp_y
+have step3_subresult18: "tanglerel_equiv (Abs_diagram ((x1)∘(basic (e2⊗y1))∘(basic (b0⊗(e1⊗w4)))∘
+a0))
+ (Abs_diagram (((x1)∘(basic y1))∘(basic (e2 ⊗ (e1 ⊗ w4)))∘ a0))" using temp_x temp_y step3_subresult17
  by auto
- 
-have step3_subresult13:  "tanglerel_equiv (Abs_diagram ((x1)∘(basic (e2⊗y1))∘(basic (a0⊗e1⊗w4))
-∘((basic (e1⊗e3⊗w5))∘z1))) 
- (Abs_diagram ((x1)∘(basic y1)∘(basic (e2 ⊗ e1 ⊗ w1))∘((basic (e1⊗e3⊗w5))∘z1)))" 
-           using step3_subresult12 temp by auto
 
-(*Whats left- sorry cases, strands, associativity rules, completing this proof and other meta cases*)
-(*
-definition tanglerel_compbelow_centerright::"diagram ⇒ diagram ⇒ bool"
-where
-tanglerel_compbelow_centerright x y ≡ ∃y1.∃w1.∃w2.∃A.∃B.∃y2.((x = Abs_diagram
- ((y1)∘(basic (A⊗w1))∘(basic (B⊗w2))∘(y2)))∧ (y = Abs_diagram ((y1)∘
-(basic (w1))∘(basic (A⊗w2))∘(y2)))
-∧((snd (count w1)) = (fst (count w2)))
-∧((fst (count A)) = 0)
-∧(strands B))"
+have step3: 
+"tanglerel_equiv (Abs_diagram ((x1)∘(basic (e2⊗y1))∘(basic (e1⊗e1⊗e1⊗w4))∘(basic (e1⊗e3⊗w4))∘z1))
+ (Abs_diagram (((x1)∘(basic y1))∘(basic (e2 ⊗ z4))∘ (basic (e1⊗e3⊗w4))∘z1))" 
+using temp temp_w step3_subresult18 leftright_associativity w_subst step2_subresult1 
+ by auto
 
- "x = (Abs_diagram (x2 ∘(basic (e2⊗e1⊗w4))∘(basic (e1⊗e3⊗w4))∘z1)
-∃y1.∃y2.∃w1.∃w2.(x = Abs_diagram (y1 ∘ (basic (e2 ⊗ e1 ⊗ w1)) ∘ (basic (e1 ⊗ e3 ⊗ w2)) ∘ y2))"
- using temp_a by auto*)
+(*combining steps*)
+                      
+have combine1: 
+"tanglerel_equiv (Abs_diagram (x1∘basic y1∘(basic (e2⊗z4))∘(basic (e1⊗e3⊗w4))∘z1)) 
+                            (Abs_diagram (x1 ∘ basic y1 ∘z1))" 
+               using step1 step2 rtranclp_trans tanglerel_equiv_def by metis
 
-(*
-have "(Abs_diagram (x2 ∘(basic (e1⊗w4))∘(basic (e1 ⊗w4))∘z1)) = 
-(Abs_diagram (x1∘(basic (e2⊗y1)∘(basic (e1⊗e1⊗w4))∘(basic (e3 ⊗w4))∘z1))"
-have "strands (e1 ⊗ e1 ⊗ w4)"
-  
+have combine2:"tanglerel_equiv (Abs_diagram ((x1)∘(basic (e2⊗y1))∘(basic (e1⊗e1⊗z4))∘(basic (e1⊗e3⊗w4))∘z1))
+             (Abs_diagram (x1 ∘ basic y1 ∘z1))" 
+               using step3 combine1 tanglerel_equiv_def rtranclp_trans
+               E compose_leftassociativity leftright_associativity 
+               step2 step2_subresult1 step2_subresult2 step3_subresult17 subresult_equiv3 
+               temp temp_b temp_w temp_x temp_y w_subst
+               by (metis) 
 
-have "a = Abs_diagram (z ∘ z1)" by (simp add: subst D)
-moreover have "tanglerel_compress_null (Abs_diagram (z∘(basic C)∘z1)) a" 
-             unfolding tanglerel_compress_null_def using A B by (metis calculation)
-moreover have "tanglerel_compress_null (Abs_diagram (z∘(basic C)∘(basic C)∘z1)) 
-                   (Abs_diagram (z∘(basic C)∘z1))" 
-             unfolding tanglerel_compress_null_def using A B by auto 
-moreover have "tanglerel_equiv (Abs_diagram (z∘(basic C)∘(basic C)∘z1)) a" unfolding tanglerel_equiv_def rtrancl_def
- by (metis (full_types) calculation(2) calculation(3) r_into_rtranclp rtranclp.rtrancl_into_rtrancl 
-tanglerel_compress_def tanglerel_def)"
-*)
-
-
-(*substitution theorems-
-
-have subresult_main4: 
-"(Abs_diagram (x3∘(basic z4)∘z1)) = (Abs_diagram (x2 ∘ (basic z4) ∘(basic z4)∘z1))"
-by (simp add: subst E)
-
-
-have subresult_main5:" 
-(Abs_diagram (x2 ∘ (basic z4) ∘(basic z4)∘z1))=(Abs_diagram (x1 ∘ (basic y1) ∘ (basic z4) ∘(basic z4)∘z1)) "
-by (simp add: subst D)
-
-
-have subresult_main6:" 
-(Abs_diagram (x2 ∘ z1))=(Abs_diagram (x1 ∘ (basic y1) ∘ z1)) "
-by (simp add: subst D)
-
-
-have subresult_step1: 
-"tanglerel_equiv (Abs_diagram (x1∘(basic y1)∘z1)) (Abs_diagram (x1 ∘(basic y1) ∘(basic z4) ∘(basic z4)∘z1))"
-using subresult_main3 subresult_main4 subresult_main5 subresult_main6 by auto
-*)
